WIP: Introduce let polymorphism

Defs.thy
@@ -2,26 +2,37 @@ theory Defs
 imports Main "Nominal2.Nominal2" "HOL-Eisbach.Eisbach"
 begin
 
-atom_decl "name"
+atom_decl "var"
+atom_decl "tyvar"
+
 nominal_datatype "\<tau>" =
-  TyUnit
- | TyArrow "\<tau>" "\<tau>"  ("_ \<rightarrow> _" 50)
+   TyUnit
+   | TyVar "tyvar"
+   | TyArrow "\<tau>" "\<tau>"  ("_ \<rightarrow> _" 50)
+
+nominal_datatype "\<sigma>" =
+  TyMono "\<tau>"
+| TyForall a::"tyvar" t::"\<sigma>" binds a in t
 
 nominal_datatype "term" =
-   Var "name"
- | Lam x::"name" "\<tau>" e::"term" binds x in e  ("\<lambda> _ : _ . _" 50)
+   Var "var"
+ | Lam x::"var" "\<tau>" e::"term" binds x in e  ("\<lambda> _ : _ . _" 50)
  | App "term" "term"
  | Unit
- | Let x::"name" "term" e2::"term" binds x in e2
+ | Let x::"var" "term" e2::"term" binds x in e2
 
-type_synonym "\<Gamma>" = "(name * \<tau>) list"
+type_synonym "\<Gamma>" = "(var * \<sigma>) list"
 
 declare term.fv_defs[simp]
+declare \<tau>.fv_defs[simp]
+declare \<sigma>.fv_defs[simp]
 
-lemma no_vars_in_ty[simp]: "atom x \<sharp> (ty :: \<tau>)"
+lemma no_vars_in_ty[simp]: "atom (x :: var) \<sharp> (ty :: \<tau>)"
   by (induction ty rule: \<tau>.induct) auto
+lemma no_vars_in_ty2[simp]: "atom (x :: var) \<sharp> (ty :: \<sigma>)"
+  by (induction ty rule: \<sigma>.induct) auto
 
-nominal_function isin :: "name * \<tau> \<Rightarrow> \<Gamma> \<Rightarrow> bool" (infixr "\<in>" 80) where
+nominal_function isin :: "var * \<sigma> \<Rightarrow> \<Gamma> \<Rightarrow> bool" (infixr "\<in>" 80) where
   "isin _ [] = False"
 | "isin (x, t) ((y, t')#xs) = (if x = y then t = t' else isin (x, t) xs)"
        apply (all_trivials)
@@ -33,15 +44,15 @@ nominal_termination (eqvt) by lexicographic_order
 
 (** subrules *)
 nominal_function
-is_v_of_e :: "term => bool"
+is_value :: "term => bool"
 where
-"is_v_of_e (Var x) = (False)"
-| "is_v_of_e (\<lambda> x : \<tau> . e) = ((True))"
-| "is_v_of_e (App e1 e2) = (False)"
-| "is_v_of_e Unit = ((True))"
-| "is_v_of_e (Let x e1 e2) = (False)"
+"is_value (Var x) = (False)"
+| "is_value (\<lambda> x : \<tau> . e) = ((True))"
+| "is_value (App e1 e2) = (False)"
+| "is_value Unit = ((True))"
+| "is_value (Let x e1 e2) = (False)"
   apply (all_trivials)
-  apply (simp add: eqvt_def is_v_of_e_graph_aux_def)
+  apply (simp add: eqvt_def is_value_graph_aux_def)
   using term.exhaust by blast
 nominal_termination (eqvt)
   by lexicographic_order
@@ -58,7 +69,7 @@ method pat_comp_aux =
 
 (** substitutions *)
 nominal_function
-subst_term :: "term => name => term => term"
+subst_term :: "term => var => term => term"
 where
 "subst_term e_5 x5 (Var x) = ((if x=x5 then e_5 else (Var x)))"
 | "atom x \<sharp> (x5, e_5) \<Longrightarrow> subst_term e_5 x5 (\<lambda> x : \<tau> . e) = (Lam x \<tau> (subst_term e_5 x5 e))"
@@ -76,33 +87,70 @@ where
   done
 nominal_termination (eqvt) by lexicographic_order
 
+nominal_function subst_type :: "\<tau> \<Rightarrow> tyvar \<Rightarrow> \<tau> \<Rightarrow> \<tau>" where
+  "subst_type t a TyUnit = TyUnit"
+| "subst_type t a (TyArrow \<tau>1 \<tau>2) = TyArrow (subst_type t a \<tau>1) (subst_type t a \<tau>2)"
+| "subst_type t a (TyVar y) = (if a = y then t else TyVar y)"
+          apply all_trivials
+     apply (auto simp: eqvt_def subst_type_graph_aux_def)
+  by (meson \<tau>.strong_exhaust)
+nominal_termination (eqvt) by lexicographic_order
+
+nominal_function subst_types :: "(tyvar * \<tau>) list \<Rightarrow> \<tau> \<Rightarrow> \<tau>" where
+  "subst_types [] t = t"
+| "subst_types ((a, \<tau>)#xs) t = subst_types xs (subst_type \<tau> a t)"
+       apply all_trivials
+    apply (auto simp: eqvt_def subst_types_graph_aux_def)
+  by (metis neq_Nil_conv surj_pair)
+nominal_termination (eqvt) by lexicographic_order
+
 lemma fresh_subst_term: "\<lbrakk> atom z \<sharp> s ; z = y \<or> atom z \<sharp> t \<rbrakk> \<Longrightarrow> atom z \<sharp> subst_term s y t"
   by (nominal_induct t avoiding: z y s rule: term.strong_induct) auto
 
+nominal_function split_vars :: "\<sigma> \<Rightarrow> tyvar list * \<tau>" where
+  "split_vars (TyMono \<tau>) = ([], \<tau>)"
+| "split_vars (TyForall a \<sigma>) = (let (xs, \<tau>) = split_vars \<sigma> in (a#xs, \<tau>))"
+       apply (auto simp: eqvt_def split_vars_graph_aux_def)
+   apply (meson \<sigma>.strong_exhaust)
+  apply (auto split: prod.splits)
+  sorry
+nominal_termination (eqvt) by lexicographic_order
+
+definition ty_leq :: "\<sigma> \<Rightarrow> \<sigma> \<Rightarrow> bool" ("_ \<sqsubseteq> _" 50) where
+  "ty_leq \<sigma> \<sigma>' = (
+    let (as, \<tau>) = split_vars \<sigma> in
+    let (bs, \<tau>') = split_vars \<sigma>' in
+    (atom ` set bs) \<sharp>* \<sigma> \<and> (\<exists>ts. \<tau>' = subst_types (zip as ts) \<tau>)
+  )"
+
 (** definitions *)
 (* defns Jwf *)
-inductive T :: "\<Gamma> \<Rightarrow> term \<Rightarrow> \<tau> \<Rightarrow> bool"
-and   "T'" :: "\<Gamma> => term => \<tau> =>  bool" ("_ \<turnstile> _ : _" 50)
+inductive T :: "\<Gamma> \<Rightarrow> term \<Rightarrow> \<sigma> \<Rightarrow> bool"
+and   "T'" :: "\<Gamma> => term => \<sigma> =>  bool" ("_ \<turnstile> _ : _" 50)
 where
   "(\<Gamma> \<turnstile> e : \<tau>) == T (\<Gamma>) (e) (\<tau>)"
 
 | (* defn T *)
 
-T_UnitI: "(\<Gamma> \<turnstile> Unit : TyUnit)"
+T_UnitI: "(\<Gamma> \<turnstile> Unit : TyMono TyUnit)"
 
-| T_VarI: "\<lbrakk> isin ( x ,  \<tau> )  \<Gamma> \<rbrakk> \<Longrightarrow>
-(\<Gamma> \<turnstile> (Var x) : \<tau>)"
+| T_VarI: "\<lbrakk> isin ( x ,  \<sigma> )  \<Gamma> \<rbrakk> \<Longrightarrow>
+(\<Gamma> \<turnstile> (Var x) : \<sigma>)"
 
-| T_AbsI: "\<lbrakk>atom x \<sharp> \<Gamma> ; ( ( x ,  \<tau>1 ) # \<Gamma>  \<turnstile> e : \<tau>2)\<rbrakk> \<Longrightarrow>
-(\<Gamma> \<turnstile>  (\<lambda> x : \<tau>1 . e)  : (\<tau>1 \<rightarrow> \<tau>2))"
+| T_AbsI: "\<lbrakk>atom (x :: var) \<sharp> \<Gamma> ; ( ( x ,  TyMono \<tau>1 ) # \<Gamma>  \<turnstile> e : TyMono \<tau>2)\<rbrakk> \<Longrightarrow>
+(\<Gamma> \<turnstile>  (\<lambda> x : \<tau>1 . e)  : TyMono (\<tau>1 \<rightarrow> \<tau>2))"
 
-| T_AppI: "\<lbrakk>(\<Gamma> \<turnstile> e1 : (\<tau>1 \<rightarrow> \<tau>2)) ;
-(\<Gamma> \<turnstile> e2 : \<tau>1)\<rbrakk> \<Longrightarrow>
-(\<Gamma> \<turnstile> (App e1 e2) : \<tau>2)"
+| T_AppI: "\<lbrakk>(\<Gamma> \<turnstile> e1 : TyMono (\<tau>1 \<rightarrow> \<tau>2)) ;
+(\<Gamma> \<turnstile> e2 : TyMono \<tau>1)\<rbrakk> \<Longrightarrow>
+(\<Gamma> \<turnstile> (App e1 e2) : TyMono \<tau>2)"
 
 | T_LetI: "\<lbrakk>atom x \<sharp> (\<Gamma>, e1) ;
-( ( x ,  \<tau>1 ) # \<Gamma>  \<turnstile> e2 : \<tau>2) ; (\<Gamma> \<turnstile> e1 : \<tau>1)\<rbrakk> \<Longrightarrow>
-(\<Gamma> \<turnstile>  (Let x e1 e2)  : \<tau>2)"
+( ( x ,  \<sigma> ) # \<Gamma>  \<turnstile> e2 : TyMono \<tau>) ; (\<Gamma> \<turnstile> e1 : \<sigma>)\<rbrakk> \<Longrightarrow>
+(\<Gamma> \<turnstile>  (Let x e1 e2)  : TyMono \<tau>)"
+
+| T_InsI: "\<lbrakk> \<Gamma> \<turnstile> e : \<sigma>' ; \<sigma>' \<sqsubseteq> \<sigma> \<rbrakk> \<Longrightarrow> \<Gamma> \<turnstile> e : \<sigma>"
+
+| T_GenI: "\<lbrakk> \<Gamma> \<turnstile> e : \<sigma> ; atom (a :: tyvar) \<sharp> \<Gamma> \<rbrakk> \<Longrightarrow> \<Gamma> \<turnstile> e : TyForall a \<sigma>"
 
 lemma fresh_not_isin: "atom x \<sharp> \<Gamma> \<Longrightarrow> \<nexists>t'. isin (x, t') \<Gamma>"
   by (induction \<Gamma>) (auto simp: fresh_Pair fresh_Cons fresh_at_base(2))
@@ -122,17 +170,17 @@ where
 
 | (* defn Step *)
 
-ST_BetaI: "\<lbrakk>is_v_of_e v\<rbrakk> \<Longrightarrow>
+ST_BetaI: "\<lbrakk>is_value v\<rbrakk> \<Longrightarrow>
 ((App  (\<lambda> x : \<tau> . e)  v) \<longrightarrow>  subst_term  v   x   e )"
 
 | ST_AppI: "\<lbrakk>(e1 \<longrightarrow> e2)\<rbrakk> \<Longrightarrow>
 ((App e1 e) \<longrightarrow> (App e2 e))"
 
-| ST_App2I: "\<lbrakk>is_v_of_e v ;
+| ST_App2I: "\<lbrakk>is_value v ;
 (e1 \<longrightarrow> e2)\<rbrakk> \<Longrightarrow>
 ((App v e1) \<longrightarrow> (App v e2))"
 
-| ST_SubstI: "\<lbrakk>is_v_of_e v\<rbrakk> \<Longrightarrow>
+| ST_SubstI: "\<lbrakk>is_value v\<rbrakk> \<Longrightarrow>
 ((Let x v e) \<longrightarrow>  subst_term  v   x   e )"
 
 | ST_LetI: "\<lbrakk>(e1 \<longrightarrow> e2)\<rbrakk> \<Longrightarrow>
